Even more refactoring

fairness/examples/choose_nat/choose_nat.v
@@ -19,10 +19,8 @@ Set Default Proof Using "Type".
 Definition decr_loop_prog (l : loc) : val :=
   rec: "go" <> :=
     let: "x" := !#l in
-    if: "x" = #1
-    then #l <- ("x" - #1)
+    if: "x" = #1 then #l <- ("x" - #1)
     else #l <- ("x" - #1);; "go" #().
-
 Definition choose_nat_prog (l : loc) : val :=
   λ: <>,
      #l <- (ChooseNat + #1);;
@@ -38,32 +36,17 @@ Definition CN_Z (cn : CN) : Z :=
   | N n => n
   end.
 
-(** Inverse mapping of program state to model state *)
-Definition Z_CN (v : val) : CN :=
-  match v with
-  | LitV (LitInt z) =>
-      match z with
-      | Z0 => N 0
-      | Zpos p => N (Pos.to_nat p)
-      | Zneg _ => Start         (* Error case when z < -1 *)
-      end
-  | _ => Start                  (* Error case *)
-  end.
-
-Lemma Z_CN_CN_Z cn : Z_CN #(CN_Z cn) = cn.
-Proof. destruct cn; [done|]; destruct n; [done|]=> /=; f_equal; lia. Qed.
-
 #[global] Instance CN_eqdec: EqDecision CN.
 Proof. solve_decision. Qed.
 
 #[global] Instance CN_inhabited: Inhabited CN.
 Proof. exact (populate Start). Qed.
 
-Inductive cntrans : CN -> option unit -> CN -> Prop :=
+Inductive cntrans : CN → option unit → CN -> Prop :=
 | start_trans n : cntrans Start (Some ()) (N n)
 | decr_trans n : cntrans (N $ S n) (Some ()) (N n).
 
-(** Free construction of the active labels on each state by [cntrans] *)
+(* Free construction of the active labels on each state by [cntrans] *)
 Definition cn_live_roles (cn : CN) : gset unit :=
   match cn with N 0 => ∅ | _ => {[ () ]} end.
 
@@ -81,232 +64,11 @@ Proof.
           |}).
 Defined.
 
-Definition cn_model : LiveModel heap_lang cn_fair_model :=
-  {| fuel_limit _ := 40%nat |}.
-
-Class choose_natG Σ := ChooseNatG {
-  choose_nat_G :> inG Σ (excl_authR ZO);
-}.
-
-Definition choose_natΣ : gFunctors :=
-  #[ heapΣ cn_fair_model; GFunctor (excl_authR ZO) ].
-
-Global Instance subG_choosenatΣ {Σ} :
-  subG choose_natΣ Σ → choose_natG Σ.
-Proof. solve_inG. Qed.
-
-Definition Ns := nroot .@ "choose_nat".
-
-Section proof.
-  Context `{!heapGS Σ cn_fair_model cn_model, choose_natG Σ}.
-
-  Definition choose_nat_inv_inner (γ : gname) (l:loc) : iProp Σ :=
-    ∃ (cn:CN), frag_model_is cn ∗ l ↦ #(CN_Z cn) ∗ own γ (●E (CN_Z cn)).
-
-  Definition choose_nat_inv (γ : gname) (l:loc) :=
-    inv Ns (choose_nat_inv_inner γ l).
-
-  Lemma decr_loop_spec γ tid l (n:nat) (f:nat) :
-    7 ≤ f → f ≤ 38 →
-    choose_nat_inv γ l -∗
-    {{{ has_fuel tid () f ∗ frag_free_roles_are ∅ ∗
-        own γ (◯E (Z.of_nat (S n))) }}}
-      decr_loop_prog l #() @ tid ; ⊤
-    {{{ RET #(); tid ↦M ∅ }}}.
-  Proof.
-    iIntros (Hle1 Hle2) "#IH".
-    iIntros "!>" (Φ) "(Hf & Hr & Hm) HΦ".
-    iInduction n as [|n] "IHn".
-    { wp_lam.
-      (* Load - with invariant *)
-      wp_bind (Load _).
-      iApply wp_atomic.
-      iInv Ns as ">HI" "Hclose".
-      iDestruct "HI" as (cn) "(Hs & Hl & Hcn)".
-      iDestruct (own_valid_2 with "Hcn Hm") as %Hvalid%excl_auth_agree_L.
-      iModIntro.
-      wp_load.
-      iModIntro.
-      iMod ("Hclose" with "[Hs Hl Hcn]") as "_"; [ iExists _; iFrame | ].
-      iModIntro.
-      rewrite Hvalid. clear cn Hvalid.
-      (* Store - with invariant *)
-      wp_pures.
-      replace (Z.of_nat 1 - 1)%Z with 0%Z by lia.
-      wp_bind (Store _ _).
-      iApply wp_atomic.
-      iInv Ns as ">HI" "Hclose".
-      iDestruct "HI" as (cn) "(Hs & Hl & Hcn)".
-      iDestruct (own_valid_2 with "Hcn Hm") as %Hvalid%excl_auth_agree_L.
-      iModIntro.
-      assert (cn = N 1) as ->.
-      { destruct cn; inversion Hvalid. by simplify_eq. }
-      iApply (wp_store_step_singlerole _ _ (():fmrole cn_fair_model) (f - 7) (f-3)
-               with "[$Hl $Hs $Hr Hf]").
-      { simpl. lia. }
-      { constructor. }
-      { set_solver. }
-      { replace (f - 1 - 1 - 1 - 1 - 1 - 1 - 1)%nat with (f - 7)%nat by lia.
-        by rewrite has_fuel_fuels. }
-      iIntros "!> (Hl & Hs & Hr & Hf)".
-      iMod (own_update_2 _ _ _ with "Hcn Hm") as "[Hcn Hm]".
-      { apply (excl_auth_update _ _ 0%Z). }
-      iMod ("Hclose" with "[Hs Hl Hcn]") as "_".
-      { iExists (N 0). iFrame. }
-      iModIntro.
-      simpl.
-      destruct (decide (() ∈ ∅)); [set_solver|].
-      by iApply "HΦ". }
-    wp_lam.
-    wp_bind (Load _).
-    iApply wp_atomic.
-    iInv Ns as ">HI" "Hclose".
-    iModIntro.
-    iDestruct "HI" as (cn) "(Hs & Hl & Hcn)".
-    wp_load.
-    iDestruct (own_valid_2 with "Hcn Hm") as %Hvalid%excl_auth_agree_L.
-    iModIntro. iMod ("Hclose" with "[Hs Hl Hcn]") as "_".
-    { iExists _. iFrame. }
-    iModIntro.
-    rewrite Hvalid. clear cn Hvalid.
-    wp_pures.
-    case_bool_decide as Heq; [inversion Heq; lia|clear Heq].
-    wp_pures.
-    replace (Z.of_nat (S (S n))  - 1)%Z with (Z.of_nat (S n)) %Z by lia.
-    (* Store - with invariant *)
-    wp_bind (Store _ _).
-    iApply wp_atomic.
-    iInv Ns as ">HI" "Hclose".
-    iModIntro.
-    iDestruct "HI" as (cn) "(Hs & Hl & Hcn)".
-    iDestruct (own_valid_2 with "Hcn Hm") as %Hvalid%excl_auth_agree_L.
-    assert (cn = N (S (S n))) as ->.
-    { destruct cn; inversion Hvalid. by simplify_eq. }
-    iApply (wp_store_step_singlerole _ _ (():fmrole cn_fair_model) (f - 7)
-                                     (f+2) with "[$Hl $Hs $Hr Hf]").
-    { simpl. lia. }
-    { constructor. }
-    { set_solver. }
-    { replace (f - 1 - 1 - 1 - 1 - 1 - 1 - 1)%nat with (f - 7)%nat by lia.
-      rewrite has_fuel_fuels. done. }
-    iIntros "!> (Hl & Hs & Hr & Hf)".
-    iMod (own_update_2 _ _ _ with "Hcn Hm") as "[Hcn Hm]".
-    { apply (excl_auth_update _ _ (Z.of_nat (S n))%Z). }
-    iMod ("Hclose" with "[Hs Hl Hcn]") as "_".
-    { iExists (N (S n)). iFrame. }
-    iModIntro.
-    simpl. destruct (decide (() ∈ {[()]})); [|set_solver].
-    wp_pures.
-    replace (f + 2 - 1 - 1)%nat with f by lia.
-    by iApply ("IHn" with "Hf Hr Hm").
-  Qed.
-
-  Lemma choose_nat_spec γ l tid (f:nat) :
-    12 ≤ f → f ≤ 40 →
-    choose_nat_inv γ l -∗
-    {{{ has_fuel tid () f ∗ frag_free_roles_are ∅ ∗ own γ (◯E (-1)%Z) }}}
-      choose_nat_prog l #() @ tid
-    {{{ RET #(); tid ↦M ∅ }}}.
-  Proof.
-    iIntros (Hle1 Hle2) "#IH".
-    iIntros "!>" (Φ) "(Hf & Hr & Hm) HΦ".
-    wp_lam.
-    wp_bind ChooseNat.
-    iApply (wp_choose_nat_nostep _ _ _ {[() := (f - 2)%nat]} with "[Hf]").
-    { set_solver. }
-    { rewrite -has_fuel_fuels_S has_fuel_fuels.
-      replace (S (f - 2))%nat with (f - 1)%nat by lia. done. }
-    iIntros "!>" (n) "Hf".
-    wp_pures.
-    (* Store - with invariant *)
-    wp_bind (Store _ _).
-    iApply wp_atomic.
-    iInv Ns as ">HI" "Hclose".
-    iModIntro.
-    iDestruct "HI" as (cn) "(Hs & Hl & Hcn)".
-    iDestruct (own_valid_2 with "Hcn Hm") as %Hvalid%excl_auth_agree_L.
-    assert (cn = Start) as ->.
-    { destruct cn; inversion Hvalid; [done|]. lia. }
-    iApply (wp_store_step_singlerole _ _ (():fmrole cn_fair_model)
-                                     (f - 3) (f-2) _ _ (N (S n))
-             with "[$Hl $Hs $Hr Hf]").
-    { simpl. lia. }
-    { constructor. }
-    { set_solver. }
-    { replace (f - 2 - 1)%nat with (f - 3)%nat by lia.
-      rewrite has_fuel_fuels. done. }
-    iIntros "!> (Hl & Hs & Hr & Hf)".
-    iMod (own_update_2 _ _ _ with "Hcn Hm") as "[Hcn Hm]".
-    { apply (excl_auth_update _ _ (Z.of_nat (S n))%Z). }
-    iMod ("Hclose" with "[Hs Hl Hcn]") as "_".
-    { replace (Z.of_nat n + 1)%Z with (Z.of_nat (S n)) by lia.
-      iExists (N (S n)). iFrame. }
-    iModIntro.
-    simpl. destruct (decide (() ∈ {[()]})); [|set_solver].
-    wp_pures.
-    rewrite -has_fuel_fuels.
-    by iApply (decr_loop_spec with "IH [$Hm $Hr $Hf]"); [lia|lia|].
-  Qed.
-
-End proof.
-
-Definition ξ_cn (l:loc) (extr : execution_trace heap_lang)
-           (auxtr : finite_trace cn_fair_model (option unit)) :=
-  ∃ (cn:CN), (trace_last extr).2.(heap) !!! l = #(CN_Z cn) ∧
-             (trace_last auxtr) = cn.
-
-(** Derive that program is related to model by [ξ_cn l] *)
-Lemma choose_nat_sim l :
-  continued_simulation
-    (sim_rel_with_user cn_model (ξ_cn l))
-    (trace_singleton ([choose_nat_prog l #()],
-                        {| heap := {[l:=#-1]};
-                           used_proph_id := ∅ |}))
-    (trace_singleton (initial_ls (LM := cn_model) Start 0%nat)).
-Proof.
-  assert (heapGpreS choose_natΣ cn_fair_model cn_model) as HPreG.
-  { apply _. }
-  eapply (strong_simulation_adequacy (Mdl := cn_fair_model)
-            choose_natΣ NotStuck _ _ _ ∅); [|set_solver|].
-  { clear.
-    apply rel_finitary_sim_rel_with_user_ξ.
-    intros extr atr c' oζ.
-    eapply finite_smaller_card_nat=> /=.
-    eapply (in_list_finite [(Z_CN (heap c'.2 !!! l), None);
-                            (Z_CN (heap c'.2 !!! l), Some ())]).
-    (* TODO: Figure out why this does not unify with typeclass *)
-    Unshelve. 2: intros x; apply make_proof_irrel.
-    intros [cn o] [cn' [Hextr Hatr]].
-    rewrite Hextr Z_CN_CN_Z -Hatr. destruct o; [destruct u|]; set_solver. }
-  iIntros (?) "!> Hσ Hs Hr Hf".
-  iMod (own_alloc) as (γ) "He"; [apply (excl_auth_valid (-1)%Z)|].
-  iDestruct "He" as "[He● He○]".
-  iMod (inv_alloc Ns ⊤ (choose_nat_inv_inner γ l) with "[He● Hσ Hs]") as "#IH".
-  { iIntros "!>". iExists _. iFrame. by rewrite big_sepM_singleton. }
-  iModIntro.
-  iSplitL.
-  { iApply (choose_nat_spec _ _ _ 40 with "IH [Hr Hf He○]");
-      [lia|lia| |by eauto]=> /=.
-    replace (∅ ∖ {[()]}) with (∅:gset unit) by set_solver.
-    rewrite has_fuel_fuels gset_to_gmap_set_to_map. iFrame. }
-  iIntros (ex atr c Hvalid Hex Hatr Hends Hξ Hstuck) "Hσ".
-  iInv Ns as ">H".
-  iDestruct "H" as (cn) "(Hf & Hl & H●)".
-  iDestruct "Hσ" as (Hvalid') "[Hσ Hs]".
-  iDestruct (gen_heap_valid with "Hσ Hl") as %Hlookup%lookup_total_correct.
-  iDestruct (model_agree' with "Hs Hf") as %Hlast.
-  iModIntro. iSplitL; [by iExists _; iFrame|].
-  iApply fupd_mask_intro; [set_solver|]. iIntros "_".
-  iPureIntro. exists cn.
-  split; [done|].
-  subst. by destruct atr.
-Qed.
-
-(** Show that model is fairly terminating *)
+(** Show that the model is fairly terminating *)
 
 Inductive cn_order : CN → CN → Prop :=
   | cn_order_Start cn : cn_order cn Start
-  | cn_order_N (n1 n2:nat) : n1 ≤ n2 → cn_order (N n1) (N n2).
+  | cn_order_N (n1 n2 : nat) : n1 ≤ n2 → cn_order (N n1) (N n2).
 
 Local Instance the_order_po: PartialOrder cn_order.
 Proof.
@@ -372,12 +134,251 @@ Next Obligation.
   - inversion Htrans; simplify_eq. constructor. lia.
 Qed.
 
-Theorem choose_nat_terminates l (extr : extrace)
-        (Hexfirst : trfirst extr = ([choose_nat_prog l #()],
-                                      {| heap := {[l:=#-1]};
-                                         used_proph_id := ∅ |})) :
+Definition cn_model : LiveModel heap_lang cn_fair_model :=
+  {| fuel_limit _ := 40%nat |}.
+
+(** Set up necessary RA constructions *)
+Class choose_natG Σ := ChooseNatG { choose_nat_G :> inG Σ (excl_authR ZO) }.
+
+Definition choose_natΣ : gFunctors :=
+  #[ heapΣ cn_fair_model; GFunctor (excl_authR ZO) ].
+
+Global Instance subG_choosenatΣ {Σ} : subG choose_natΣ Σ → choose_natG Σ.
+Proof. solve_inG. Qed.
+
+Definition Ns := nroot .@ "choose_nat".
+
+Section proof.
+  Context `{!heapGS Σ cn_fair_model cn_model, choose_natG Σ}.
+
+  Definition choose_nat_inv_inner (γ : gname) (l:loc) : iProp Σ :=
+    ∃ (cn:CN), frag_model_is cn ∗ l ↦ #(CN_Z cn) ∗ own γ (●E (CN_Z cn)).
+
+  Definition choose_nat_inv (γ : gname) (l:loc) :=
+    inv Ns (choose_nat_inv_inner γ l).
+
+  Lemma decr_loop_spec γ tid l (n:nat) (f:nat) :
+    7 ≤ f → f ≤ 38 →
+    choose_nat_inv γ l -∗
+    {{{ has_fuel tid () f ∗ frag_free_roles_are ∅ ∗
+        own γ (◯E (Z.of_nat (S n))) }}}
+      decr_loop_prog l #() @ tid ; ⊤
+    {{{ RET #(); tid ↦M ∅ }}}.
+  Proof.
+    iIntros (Hle1 Hle2) "#IH".
+    iIntros "!>" (Φ) "(Hf & Hr & Hm) HΦ".
+    iInduction n as [|n] "IHn".
+    { wp_lam.
+      (* Load - with invariant *)
+      wp_bind (Load _).
+      iApply wp_atomic.
+      iInv Ns as ">HI" "Hclose".
+      iDestruct "HI" as (cn) "(Hs & Hl & Hcn)".
+      iDestruct (own_valid_2 with "Hcn Hm") as %Hvalid%excl_auth_agree_L.
+      iModIntro.
+      wp_load.
+      iModIntro.
+      iMod ("Hclose" with "[Hs Hl Hcn]") as "_"; [ iExists _; iFrame | ].
+      iModIntro.
+      rewrite Hvalid. clear cn Hvalid.
+      (* Store - with invariant *)
+      wp_pures.
+      replace (Z.of_nat 1 - 1)%Z with 0%Z by lia.
+      wp_bind (Store _ _).
+      iApply wp_atomic.
+      iInv Ns as ">HI" "Hclose".
+      iDestruct "HI" as (cn) "(Hs & Hl & Hcn)".
+      iDestruct (own_valid_2 with "Hcn Hm") as %Hvalid%excl_auth_agree_L.
+      iModIntro.
+      assert (cn = N 1) as ->.
+      { destruct cn; inversion Hvalid. by simplify_eq. }
+      (* Update the model state to maintain program correspondence *)
+      iApply (wp_store_step_singlerole _ _ (():fmrole cn_fair_model) (f - 7) (f-3)
+               with "[$Hl $Hs $Hr Hf]").
+      { simpl. lia. }
+      { constructor. }
+      { set_solver. }
+      { replace (f - 1 - 1 - 1 - 1 - 1 - 1 - 1)%nat with (f - 7)%nat by lia.
+        by rewrite has_fuel_fuels. }
+      iIntros "!> (Hl & Hs & Hr & Hf)".
+      iMod (own_update_2 _ _ _ with "Hcn Hm") as "[Hcn Hm]".
+      { apply (excl_auth_update _ _ 0%Z). }
+      iMod ("Hclose" with "[Hs Hl Hcn]") as "_".
+      { iExists (N 0). iFrame. }
+      iModIntro.
+      simpl.
+      destruct (decide (() ∈ ∅)); [set_solver|].
+      by iApply "HΦ". }
+    wp_lam.
+    (* Load - with invariant *)
+    wp_bind (Load _).
+    iApply wp_atomic.
+    iInv Ns as ">HI" "Hclose".
+    iModIntro.
+    iDestruct "HI" as (cn) "(Hs & Hl & Hcn)".
+    wp_load.
+    iDestruct (own_valid_2 with "Hcn Hm") as %Hvalid%excl_auth_agree_L.
+    iModIntro. iMod ("Hclose" with "[Hs Hl Hcn]") as "_".
+    { iExists _. iFrame. }
+    iModIntro.
+    rewrite Hvalid. clear cn Hvalid.
+    wp_pures.
+    case_bool_decide as Heq; [inversion Heq; lia|clear Heq].
+    wp_pures.
+    replace (Z.of_nat (S (S n))  - 1)%Z with (Z.of_nat (S n)) %Z by lia.
+    (* Store - with invariant *)
+    wp_bind (Store _ _).
+    iApply wp_atomic.
+    iInv Ns as ">HI" "Hclose".
+    iModIntro.
+    iDestruct "HI" as (cn) "(Hs & Hl & Hcn)".
+    iDestruct (own_valid_2 with "Hcn Hm") as %Hvalid%excl_auth_agree_L.
+    assert (cn = N (S (S n))) as ->.
+    { destruct cn; inversion Hvalid. by simplify_eq. }
+    (* Update the model state to maintain program correspondence *)
+    iApply (wp_store_step_singlerole _ _ (():fmrole cn_fair_model) (f - 7)
+                                     (f+2) with "[$Hl $Hs $Hr Hf]").
+    { simpl. lia. }
+    { constructor. }
+    { set_solver. }
+    { replace (f - 1 - 1 - 1 - 1 - 1 - 1 - 1)%nat with (f - 7)%nat by lia.
+      rewrite has_fuel_fuels. done. }
+    iIntros "!> (Hl & Hs & Hr & Hf)".
+    iMod (own_update_2 _ _ _ with "Hcn Hm") as "[Hcn Hm]".
+    { apply (excl_auth_update _ _ (Z.of_nat (S n))%Z). }
+    iMod ("Hclose" with "[Hs Hl Hcn]") as "_".
+    { iExists (N (S n)). iFrame. }
+    iModIntro.
+    simpl. destruct (decide (() ∈ {[()]})); [|set_solver].
+    wp_pures.
+    replace (f + 2 - 1 - 1)%nat with f by lia.
+    by iApply ("IHn" with "Hf Hr Hm").
+  Qed.
+
+  Lemma choose_nat_spec γ l tid (f:nat) :
+    12 ≤ f → f ≤ 40 →
+    choose_nat_inv γ l -∗
+    {{{ has_fuel tid () f ∗ frag_free_roles_are ∅ ∗ own γ (◯E (-1)%Z) }}}
+      choose_nat_prog l #() @ tid
+    {{{ RET #(); tid ↦M ∅ }}}.
+  Proof.
+    iIntros (Hle1 Hle2) "#IH".
+    iIntros "!>" (Φ) "(Hf & Hr & Hm) HΦ".
+    wp_lam.
+    wp_bind ChooseNat.
+    iApply (wp_choose_nat_nostep _ _ _ {[() := (f - 2)%nat]} with "[Hf]").
+    { set_solver. }
+    { rewrite -has_fuel_fuels_S has_fuel_fuels.
+      replace (S (f - 2))%nat with (f - 1)%nat by lia. done. }
+    iIntros "!>" (n) "Hf".
+    wp_pures.
+    (* Store - with invariant *)
+    wp_bind (Store _ _).
+    iApply wp_atomic.
+    iInv Ns as ">HI" "Hclose".
+    iModIntro.
+    iDestruct "HI" as (cn) "(Hs & Hl & Hcn)".
+    iDestruct (own_valid_2 with "Hcn Hm") as %Hvalid%excl_auth_agree_L.
+    assert (cn = Start) as ->.
+    { destruct cn; inversion Hvalid; [done|]. lia. }
+    (* Update the model state to maintain program correspondence *)
+    iApply (wp_store_step_singlerole _ _ (():fmrole cn_fair_model)
+                                     (f - 3) (f-2) _ _ (N (S n))
+             with "[$Hl $Hs $Hr Hf]").
+    { simpl. lia. }
+    { constructor. }
+    { set_solver. }
+    { replace (f - 2 - 1)%nat with (f - 3)%nat by lia.
+      rewrite has_fuel_fuels. done. }
+    iIntros "!> (Hl & Hs & Hr & Hf)".
+    iMod (own_update_2 _ _ _ with "Hcn Hm") as "[Hcn Hm]".
+    { apply (excl_auth_update _ _ (Z.of_nat (S n))%Z). }
+    iMod ("Hclose" with "[Hs Hl Hcn]") as "_".
+    { replace (Z.of_nat n + 1)%Z with (Z.of_nat (S n)) by lia.
+      iExists (N (S n)). iFrame. }
+    iModIntro.
+    simpl. destruct (decide (() ∈ {[()]})); [|set_solver].
+    wp_pures.
+    rewrite -has_fuel_fuels.
+    by iApply (decr_loop_spec with "IH [$Hm $Hr $Hf]"); [lia|lia|].
+  Qed.
+
+End proof.
+
+Definition ξ_cn (l:loc) (extr : execution_trace heap_lang)
+           (auxtr : finite_trace cn_fair_model (option unit)) :=
+  ∃ (cn:CN), (trace_last extr).2.(heap) !!! l = #(CN_Z cn) ∧
+             (trace_last auxtr) = cn.
+
+(** Inverse mapping of program state to model state *)
+Definition Z_CN (v : val) : CN :=
+  match v with
+  | LitV (LitInt z) =>
+      match z with
+      | Z0 => N 0
+      | Zpos p => N (Pos.to_nat p)
+      | Zneg _ => Start         (* Error case when z < -1 *)
+      end
+  | _ => Start                  (* Error case *)
+  end.
+
+Lemma Z_CN_CN_Z cn : Z_CN #(CN_Z cn) = cn.
+Proof. destruct cn; [done|]; destruct n; [done|]=> /=; f_equal; lia. Qed.
+
+(** Derive that program is related to model by [ξ_cn l] *)
+Lemma choose_nat_sim l :
+  continued_simulation
+    (sim_rel_with_user cn_model (ξ_cn l))
+    (trace_singleton ([choose_nat_prog l #()],
+                        {| heap := {[l:=#-1]};
+                           used_proph_id := ∅ |}))
+    (trace_singleton (initial_ls (LM := cn_model) Start 0%nat)).
+Proof.
+  assert (heapGpreS choose_natΣ cn_fair_model cn_model) as HPreG.
+  { apply _. }
+  eapply (strong_simulation_adequacy (Mdl := cn_fair_model)
+            choose_natΣ NotStuck _ _ _ ∅); [|set_solver|].
+  { clear.
+    apply rel_finitary_sim_rel_with_user_ξ.
+    intros extr atr c' oζ.
+    eapply finite_smaller_card_nat=> /=.
+    eapply (in_list_finite [(Z_CN (heap c'.2 !!! l), None);
+                            (Z_CN (heap c'.2 !!! l), Some ())]).
+    (* TODO: Figure out why this does not unify with typeclass *)
+    Unshelve. 2: intros x; apply make_proof_irrel.
+    intros [cn o] [cn' [Hextr Hatr]].
+    rewrite Hextr Z_CN_CN_Z -Hatr. destruct o; [destruct u|]; set_solver. }
+  iIntros (?) "!> Hσ Hs Hr Hf".
+  iMod (own_alloc) as (γ) "He"; [apply (excl_auth_valid (-1)%Z)|].
+  iDestruct "He" as "[He● He○]".
+  iMod (inv_alloc Ns ⊤ (choose_nat_inv_inner γ l) with "[He● Hσ Hs]") as "#IH".
+  { iIntros "!>". iExists _. iFrame. by rewrite big_sepM_singleton. }
+  iModIntro.
+  iSplitL.
+  { iApply (choose_nat_spec _ _ _ 40 with "IH [Hr Hf He○]");
+      [lia|lia| |by eauto]=> /=.
+    replace (∅ ∖ {[()]}) with (∅:gset unit) by set_solver.
+    rewrite has_fuel_fuels gset_to_gmap_set_to_map. iFrame. }
+  iIntros (ex atr c Hvalid Hex Hatr Hends Hξ Hstuck) "Hσ".
+  iInv Ns as ">H".
+  iDestruct "H" as (cn) "(Hf & Hl & H●)".
+  iDestruct "Hσ" as (Hvalid') "[Hσ Hs]".
+  iDestruct (gen_heap_valid with "Hσ Hl") as %Hlookup%lookup_total_correct.
+  iDestruct (model_agree' with "Hs Hf") as %Hlast.
+  iModIntro. iSplitL; [by iExists _; iFrame|].
+  iApply fupd_mask_intro; [set_solver|]. iIntros "_".
+  iPureIntro. exists cn.
+  split; [done|].
+  subst. by destruct atr.
+Qed.
+
+Theorem choose_nat_terminates l extr :
+  trfirst extr = ([choose_nat_prog l #()],
+                    {| heap := {[l:=#-1]};
+                      used_proph_id := ∅ |}) →
   extrace_fairly_terminating extr.
 Proof.
+  intros Hexfirst.
   eapply heap_lang_continued_simulation_fair_termination; eauto.
   rewrite Hexfirst. eapply choose_nat_sim.
 Qed.
